@prefix rdf: <http://www.w3.org/1999/02/22-rdf-syntax-ns#> .
@prefix rdfs: <http://www.w3.org/2000/01/rdf-schema#> .
@prefix sesame: <http://www.openrdf.org/schema/sesame#> .
@prefix owl: <http://www.w3.org/2002/07/owl#> .
@prefix xsd: <http://www.w3.org/2001/XMLSchema#> .
@prefix fn: <http://www.w3.org/2005/xpath-functions#> .
@prefix foaf: <http://xmlns.com/foaf/0.1/> .
@prefix dc: <http://purl.org/dc/elements/1.1/> .
@prefix hint: <http://www.bigdata.com/queryHints#> .
@prefix bd: <http://www.bigdata.com/rdf#> .
@prefix bds: <http://www.bigdata.com/rdf/search#> .

<http://rs.tdwg.org/cv/status/inappropriate> <http://www.w3.org/2004/02/skos/core#hiddenLabel> "Skeleton on loan to Vertebrate Paleontology Teaching Collection from 2000 - 2005" , "Skin exchanged to St. Bonaventure University ( S. W. Eaton), St. Bonaventure, New York, for 10896, 10897, 18 May 1976 ( D S W), Deaccessioned on 2 February 2015" , "Skin in Buenos Aires: M A C N 52678" , "Skin on loan, 9 June 2004" , "Specimen in  Synoptic Collection" , "Specimen in Synoptic Collection" , "Specimen in Synoptic Collection (traded for O M N H 00800, O M N H 02639, O M N H 04941, O M H H 10426)" , "Specimen in Synoptic Collection." , "T" , "Thinning" , "This record is only a numerical placeholder. Catalog number originally assigned to fluid preserved stomach contents without specimens" , "This specimen is the same as 7961" , "Threatened" , "To be regenerated" , "Toe pad loaned for DNA extraction to Dr. Rebecca Kimball, Department of Biology, University of Florida (ZO.2014.2)" , "Toe pad loaned for DNA extraction to Dr. Samantha Wisely, KSU Conservation Genetic and Molecular Ecology Lab, Kansas State University (ZO.2011.2)" , "Toe pad loaned for DNA extraction to Dr. Samantha Wisely, KSU Conservation Genetic and Molecular Ecology Lab, Kansas State University (ZO.2011.2)x" , "Treated" , "University of Oklahoma Biological Station 191" , "Unprocessed" , "valtalajina" , "VU" ;
	<http://www.w3.org/2004/02/skos/core#inScheme> <http://rs.tdwg.org/cv/status/> ;
	<http://www.w3.org/2004/02/skos/core#prefLabel> "inappropriate"@en , "inadecuado"@es , "数值格式不符"@zh-hans , "數值格式不符"@zh-hant .

<http://rs.tdwg.org/cv/status/inappropriate.ttl> <http://purl.org/dc/terms/references> <http://rs.tdwg.org/cv/status/inappropriate> ;
	a foaf:Document ;
	rdfs:comment "Generated by Guid-O-Matic 2.0 https://github.com/baskaufs/guid-o-matic" ;
	<http://purl.org/dc/terms/modified> "2017-04-21T10:17:00.000Z"^^xsd:dateTime ;
	dc:creator "Biodiversity Information Standards (TDWG)" ;
	dc:format "text/turtle" .

<http://rs.tdwg.org/cv/status/null> <http://purl.org/dc/terms/isPartOf> <http://rs.tdwg.org/cv/status/> ;
	a <http://www.w3.org/2004/02/skos/core#Concept> ;
	rdf:value "null" ;
	rdfs:comment "Record did not include a value"@en ;
	rdfs:isDefinedBy <http://rs.tdwg.org/cv/status/> ;
	rdfs:label "no value given"@en ;
	<http://www.w3.org/2004/02/skos/core#definition> "Record did not include a value"@en , "El registro no incluye valor adecuado"@es , "该物种记录中没有可用数值"@zh-hans , "該物種記錄中沒有可用數值。"@zh-hant ;
	<http://www.w3.org/2004/02/skos/core#hiddenLabel> "NA" , "\\N" ;
	<http://www.w3.org/2004/02/skos/core#inScheme> <http://rs.tdwg.org/cv/status/> ;
	<http://www.w3.org/2004/02/skos/core#prefLabel> "no value given"@en , "sin valor"@es , "缺乏数值"@zh-hans , "缺乏數值"@zh-hant .

<http://rs.tdwg.org/cv/status/null.ttl> <http://purl.org/dc/terms/references> <http://rs.tdwg.org/cv/status/null> ;
	a foaf:Document ;
	rdfs:comment "Generated by Guid-O-Matic 2.0 https://github.com/baskaufs/guid-o-matic" ;
	<http://purl.org/dc/terms/modified> "2017-04-21T10:17:00.000Z"^^xsd:dateTime ;
	dc:creator "Biodiversity Information Standards (TDWG)" ;
	dc:format "text/turtle" .

<http://rs.tdwg.org/cv/status/pextant> <http://purl.org/dc/terms/isPartOf> <http://rs.tdwg.org/cv/status/> ;
	a <http://www.w3.org/2004/02/skos/core#Concept> ;
	rdf:value "possibly extant" ;
	rdfs:comment "There is no record of the species in the area, but the species may possibly occur."@en ;
	rdfs:isDefinedBy <http://rs.tdwg.org/cv/status/> ;
	rdfs:label "possibly extant"@en ;
	<http://www.w3.org/2004/02/skos/core#definition> "There is no record of the species in the area, but the species may possibly occur."@en , "Es fehlen Aufzeichnungen der Art im Gebiet, aber die Art könnte dort auftreten. "@de , "No hay registro de la especie en el area, pero es posible que la especie se encuentre allí"@es , "Não há registos da espécie embora possivelmente ocorra na área."@pt , "该地区没有该物种的记录，但是该物种有可能在此出现。"@zh-hans , "該地區沒有該物種的記錄，但是該物種有可能在此出現。"@zh-hant ;
	<http://www.w3.org/2004/02/skos/core#hiddenLabel> "possible breeding" , "probable breeding" ;
	<http://www.w3.org/2004/02/skos/core#inScheme> <http://rs.tdwg.org/cv/status/> ;
	<http://www.w3.org/2004/02/skos/core#prefLabel> "possibly extant"@en , "möglicherweise vorhanden"@de , "posiblemente existente"@es , "possivelmente presente"@pt , "可能现存"@zh-hans , "可能現存"@zh-hant .

<http://rs.tdwg.org/cv/status/pextant.ttl> <http://purl.org/dc/terms/references> <http://rs.tdwg.org/cv/status/pextant> ;
	a foaf:Document ;
	rdfs:comment "Generated by Guid-O-Matic 2.0 https://github.com/baskaufs/guid-o-matic" ;
	<http://purl.org/dc/terms/modified> "2017-04-07T00:20:00.000Z"^^xsd:dateTime ;
	dc:creator "Biodiversity Information Standards (TDWG)" ;
	dc:format "text/turtle" .

<http://rs.tdwg.org/cv/status/pextinct> <http://purl.org/dc/terms/isPartOf> <http://rs.tdwg.org/cv/status/> ;
	a <http://www.w3.org/2004/02/skos/core#Concept> ;
	rdf:value "possibly extinct" ;
	rdfs:comment "The species was formerly known or thought very likely to occur in the area (post 1500 AD), but it is most likely now extirpated from the area because habitat loss and/or other threats are thought likely to have extirpated the species, and there have been no confirmed recent records despite searches."@en ;
	rdfs:isDefinedBy <http://rs.tdwg.org/cv/status/> ;
	rdfs:label "possibly extinct"@en ;
	<http://www.w3.org/2004/02/skos/core#definition> "该物种曾经在该区域存在过或者很可能存在过 (公元1500年后)， 但是该物种很可能已经由于栖息地的缺失或者是其他的威胁而消失，对该地区调查后也没有发现任何确定的近期该物种出现的记录。"@zh-hans , "該物種曾經在該區域存在過或者很可能存在過 (公元1500年後)， 但是該物種很可能已經由于棲息地的缺失或者是其他的威脅而消失，對該地區調查後也沒有發現任何確定的近期該物種出現的記錄。"@zh-hant , "Se sabe de la existencia de la especie en el area en el pasado, o se cree que la especie pudo haber existido en el area, pero es muy probable que la especie no se encuentre debido a que luego de búsquedas exhaustivas, no se han producido registros recientes y la intensidad duracion de amenazas posiblemente hayan extirpado el taxón"@es , "Sabe-se que a espécie ocorreu na área ou a sua ocorrência foi tida como bastante provável mas confirmou-se que a espécie já não aí ocorre devido a procuras exaustivas serem incapazes de produzir registos recentes; a intensidade e timing das ameaças terá provavelmente extirpado o táxone."@pt , "The species was formerly known or thought very likely to occur in the area (post 1500 AD), but it is most likely now extirpated from the area because habitat loss and/or other threats are thought likely to have extirpated the species, and there have been no confirmed recent records despite searches."@en , "Von der Art war früher bekannt oder mit hoher Wahrscheinlichkeit angenommen, dass sie im Gebiet anwesend war, aber inzwischen wurde bestätigt, dass die Art dort nicht länger auftritt, aufgrund von gründlicher, aber vergeblicher, aktueller Suche, wobei es plausibel ist, dass das Taxon aufgrund der Intensität und des Zeitpunkts der Bedrohung ausgerottet sein dürfte."@de ;
	<http://www.w3.org/2004/02/skos/core#inScheme> <http://rs.tdwg.org/cv/status/> ;
	<http://www.w3.org/2004/02/skos/core#prefLabel> "possibly extinct"@en , "möglicherweise ausgestorben "@de , "possiblemente extinta"@es , "possivelmente extinta"@pt .

<http://rs.tdwg.org/cv/status/extinct> <http://www.w3.org/2004/02/skos/core#inScheme> <http://rs.tdwg.org/cv/status/> ;
	<http://www.w3.org/2004/02/skos/core#prefLabel> "extinct"@en , "ausgestorben "@de , "extinta"@es , "extinta"@pt , "灭绝"@zh-hans , "滅絕"@zh-hant .

<http://rs.tdwg.org/cv/status/extinct.ttl> <http://purl.org/dc/terms/references> <http://rs.tdwg.org/cv/status/extinct> ;
	a foaf:Document ;
	rdfs:comment "Generated by Guid-O-Matic 2.0 https://github.com/baskaufs/guid-o-matic" ;
	<http://purl.org/dc/terms/modified> "2017-04-07T00:20:00.000Z"^^xsd:dateTime ;
	dc:creator "Biodiversity Information Standards (TDWG)" ;
	dc:format "text/turtle" .

<http://rs.tdwg.org/cv/status/inappropriate> <http://purl.org/dc/terms/isPartOf> <http://rs.tdwg.org/cv/status/> ;
	a <http://www.w3.org/2004/02/skos/core#Concept> ;
	rdf:value "inappropriate" ;
	rdfs:comment "Record included a value that was inappropriate for the occurrenceStatus property"@en ;
	rdfs:isDefinedBy <http://rs.tdwg.org/cv/status/> ;
	rdfs:label "inappropriate"@en ;
	<http://www.w3.org/2004/02/skos/core#definition> "Record included a value that was inappropriate for the occurrenceStatus property"@en , "El registro incluye un valor no adecuado para la propiedad estadoOcurrencia"@es , "该物种记录中没有可用于确定出现状态的数值"@zh-hans , "該物種記錄中沒有可用于確定出現狀態的數值。"@zh-hant ;
	<http://www.w3.org/2004/02/skos/core#hiddenLabel> "1" , "10" , "11" , "3" , "5" , "6" , "8" , "9" , "4" , "7" , "(EN)" , "(NT)" , "(VU)" , "adult; red; banded 30 April 1967 (band number 515-35307); also banded were five nestlings from a box \"above the Cooksey's back stoop\", Norman, OK; it was at least one year old when banded; banded by Dr. Paul F. Nighswonger." , "Attacked" , "complet" , "CR" , "Damaged" , "DD" , "Defoliated" , "Destroyed" , "Discarded by Dr. Mayr: 18 November 1942" , "Do not loan or exchange" , "Do Not Loan or Exchange, See File on Endangered Species" , "Duplicate of E4960 (egg card cataloged separately as E4960)" , "E" , "EN" , "Exchanged to St. Bonaventure University ( S. W. Eaton), St. Bonaventure, New York, for 10896, 10897, 18 May 1976 ( D S W), Deaccessioned on 2 February 2015" , "Extraviado" , "Feathers were destructively sampled and loaned to Marie Perkins, Louisiana State University (ZO.2006.1)" , "Fellings" , "Gifted to the Carnegie Museum of Natural History (CM 135911), Deaccessioned on 2 February 2015" , "Gifted to the Cornell University Museum of Vertebrates, Deaccessioned on 2 February 2015" , "In House Loan, Specimen in Art Room.  Removed from Collections:  17 June 2002" , "In House Loan, Specimen in the Black Mesa Diorama.  Prepared for the exhibit and installed in March 2011." , "In House Loan, Specimen in the Black Mesa Diorama.  Prepared for the exhibit and installed in May 2011." , "In House Loan, Specimen in the Orientation Gallery.  Prepared by taxidermist in 2009." , "In House Loan, Specimen in the Orientation Gallery.  Removed from Collections:  February 2009." , "In House Loan, Specimen in the Orientation Gallery.  Removed from Collections: 24 June 2011." , "In House Loan, Specimen on Exhibit (Orientation Gallery). Removed from Collections in February 2009" , "In House Loan, Specimen on Exhibit (Orientation Gallery). Removed from Collections: 27 March 2009" , "In House Loan, Specimen on Exhibit at the Will Rodgers International Airport.  Removed from Collections:  25 April 2002.  Returned to Collections: 19 February 2003" , "In House Loan, Specimen on Exhibit.  Removed from Colections:  3 April 2000 (V. Byre)" , "In House Loan, Specimen on Exhibit.  Removed from Collections:  25 April 2000" , "In House Loan, Specimen on Exhibit.  Removed from Collections:  5 April 2000" , "In House Loan, Specimen on Exhibit. Removed from Collections Prior to May 2001." , "In House Loan, Specimen on Exhibit. Removed from Collections: 3 April 2000" , "In House Loan, Specimen on Exhibit. Removed from Collections: June 2002" , "In the Discovery Room from 1999 to present day" , "In the Discovery Room from 2000 to present day" , "Incidental fellings" , "incomplet" , "Killed" , "Left in the forest" , "Loan skull only for SEAM scanning project  28 November 2011 - 28 February 2012" , "Lost" , "Missing as of July 2012" , "Missing in 2000 Inventory, but Present in 1991 Inventory.  Returned to Collections: 2005" , "Missing Wing:  August 2002" , "niukasti" , "Not available for destructive sampling" , "nt" , "NT" , "On loan to Richard O. Prum, Yale Peabody Natural History Museum" , "On Loan: 9 June 2004" , "Población introducida" , "Processed" , "radan vieressä" , "rare" , "raro" , "RE" , "Record created for missing catalog number" , "Removals" , "RT" , "Salvage fellings" , "Sanitation fellings" , "Sanitation removals" .

<http://rs.tdwg.org/cv/origin/> a <http://rs.tdwg.org/dwc/terms/attributes/TermList> , <http://www.w3.org/2004/02/skos/core#ConceptScheme> ;
	rdfs:comment "For each term in this list, the controlled value (rdf:value), and definition (rdfs:comment) are normative.  Labels (rdfs:label) and comments (dcterms:description) are non-normative." , "This is a controlled vocabulary whose terms are intended to be used as values for a proposed Darwin Core term dwc:origin/dwciri:origin."@en ;
	rdfs:label "Origin Controlled Vocabulary Term List"@en ;
	<http://www.w3.org/2004/02/skos/core#hasTopConcept> <http://rs.tdwg.org/cv/origin/introduced> , <http://rs.tdwg.org/cv/origin/native> , <http://rs.tdwg.org/cv/origin/unknown> ;
	<http://www.w3.org/2004/02/skos/core#note> "This is a controlled vocabulary whose terms are intended to be used as values for a proposed Darwin Core term dwc:origin/dwciri:origin."@en ;
	<http://purl.org/dc/terms/modified> "2017-04-06"^^xsd:date ;
	<http://purl.org/dc/terms/title> "Origin Controlled Vocabulary Term List"@en .

<http://rs.tdwg.org/cv/path/> <http://purl.org/dc/terms/isPartOf> <http://rs.tdwg.org/cv/> ;
	<http://purl.org/vocab/vann/preferredNamespacePrefix> "cvpath" ;
	<http://purl.org/vocab/vann/preferredNamespaceUri> "http://rs.tdwg.org/cv/path/" ;
	a <http://rs.tdwg.org/dwc/terms/attributes/TermList> , <http://www.w3.org/2004/02/skos/core#ConceptScheme> ;
	rdfs:comment "For each term in this list, the controlled value (rdf:value), and definition (rdfs:comment) are normative.  Labels (rdfs:label) and comments (dcterms:description) are non-normative." , "This is a controlled vocabulary whose terms are intended to be used as values for the Darwin Core term dwc:establishmentMeans/dwciri:establishmentMeans."@en ;
	rdfs:label "Pathway Controlled Vocabulary Term List"@en ;
	<http://www.w3.org/2004/02/skos/core#hasTopConcept> <http://rs.tdwg.org/cv/path/100> , <http://rs.tdwg.org/cv/path/101> , <http://rs.tdwg.org/cv/path/102> , <http://rs.tdwg.org/cv/path/111> , <http://rs.tdwg.org/cv/path/124> , <http://rs.tdwg.org/cv/path/135> , <http://rs.tdwg.org/cv/path/147> , <http://rs.tdwg.org/cv/path/150> ;
	<http://www.w3.org/2004/02/skos/core#note> "This is a controlled vocabulary whose terms are intended to be used as values for the Darwin Core term dwc:establishmentMeans/dwciri:establishmentMeans."@en ;
	<http://purl.org/dc/terms/modified> "2017-04-06"^^xsd:date ;
	<http://purl.org/dc/terms/title> "Pathway Controlled Vocabulary Term List"@en .

<http://www.tdwg.org/standards/x> <http://purl.org/dc/terms/hasPart> <http://rs.tdwg.org/cv/> ;
	a <http://purl.org/dc/terms/Standard> ;
	rdfs:label "fake TDWG controlled vocabulary standard" ;
	<http://purl.org/dc/terms/description> "Placeholder standard to show how the metadata would be set up if this became part of a standard" ;
	<http://purl.org/dc/terms/publisher> <https://www.grid.ac/institutes/grid.480498.9> ;
	<http://purl.org/dc/terms/title> "fake TDWG controlled vocabulary standard" ;
	dc:publisher "Biodiversity Information Standards (TDWG)" .

<http://rs.tdwg.org/cv/status/pextinct> <http://www.w3.org/2004/02/skos/core#prefLabel> "可能灭绝"@zh-hans , "可能滅絕"@zh-hant .

<http://rs.tdwg.org/cv/status/pextinct.ttl> <http://purl.org/dc/terms/references> <http://rs.tdwg.org/cv/status/pextinct> ;
	a foaf:Document ;
	rdfs:comment "Generated by Guid-O-Matic 2.0 https://github.com/baskaufs/guid-o-matic" ;
	<http://purl.org/dc/terms/modified> "2017-05-02T12:54:00.000Z"^^xsd:dateTime ;
	dc:creator "Biodiversity Information Standards (TDWG)" ;
	dc:format "text/turtle" .

<http://rs.tdwg.org/cv/status/recentlyextinct> <http://purl.org/dc/terms/isPartOf> <http://rs.tdwg.org/cv/status/> ;
	a <http://www.w3.org/2004/02/skos/core#Concept> ;
	rdf:value "extinct post 1500" ;
	rdfs:comment "The species was formerly known or thought very likely to occur in the area (post 1500 AD), but it has been confirmed that the species no longer occurs because exhaustive searches have failed to produce recent records, and the intensity and timing of threats could plausibly have extirpated the taxon."@en ;
	rdfs:isDefinedBy <http://rs.tdwg.org/cv/status/> ;
	rdfs:label "extinct post 1500"@en ;
	<http://www.w3.org/2004/02/skos/core#broader> <http://rs.tdwg.org/cv/status/extinct> ;
	<http://www.w3.org/2004/02/skos/core#definition> "该物种曾经在该区域存在过或者很可能存在过 （公元1500年后）， 但是由于对该地区彻底调查后没有发现任何近期该物种出现的记录，并且其受到的威胁的强度和时机有根除该物种的可能性，该物种已经被确认不再存在。"@zh-hans , "該物種曾經在該區域存在過或者很可能存在過 （公元1500年後）， 但是由于對該地區徹底調查後沒有發現任何近期該物種出現的記錄，並且其受到的威脅的強度和時機有根除該物種的可能性，該物種已經被確認不再存在。"@zh-hant , "Von der Art war früher bekannt oder wurde mit hoher Wahrscheinlichkeit angenommen, dass sie im Gebiet anwesend war (nach 1500 AD), aber inzwischen wurde bestätigt, dass die Art nicht länger dort auftritt, aufgrund von gründlicher, aber vergeblicher, aktueller Suche, wobei es plausibel ist, dass das Taxon aufgrund der Intensität und des Zeitpunkts der Bedrohung ausgerottet sein dürfte."@de , "The species was formerly known or thought very likely to occur in the area (post 1500 AD), but it has been confirmed that the species no longer occurs because exhaustive searches have failed to produce recent records, and the intensity and timing of threats could plausibly have extirpated the taxon."@en , "Se sabe de la existencia de la especie en el area en el pasado, o se cree que la especie pudo haber existido en el area (despues del año 1,500), pero se ha confirmado que la especie no se encuentra debido a que luego de búsquedas exhaustivas, no se han producido registros recientes, y la intensidad duracion de amenazas posiblemente hayan extirpado el taxón"@es , "Sabe-se que a espécie ocorreu na área ou a sua ocorrência foi tida como bastante provável (após 1500 d.C.) mas confirmou-se que a espécie já não aí ocorre devido a procuras exaustivas serem incapazes de produzir registos recentes; a intensidade e timing das ameaças terá provavelmente extirpado o táxone."@pt ;
	<http://www.w3.org/2004/02/skos/core#inScheme> <http://rs.tdwg.org/cv/status/> ;
	<http://www.w3.org/2004/02/skos/core#prefLabel> "extinct post 1500"@en , "ausgestorben nach 1500 AD"@de , "extinta post 1500"@es , "extinta após 1500"@pt , "公元1500年后灭绝"@zh-hans , "公元1500年後滅絕"@zh-hant .

<http://rs.tdwg.org/cv/status/recentlyextinct.ttl> <http://purl.org/dc/terms/references> <http://rs.tdwg.org/cv/status/recentlyextinct> ;
	a foaf:Document ;
	rdfs:comment "Generated by Guid-O-Matic 2.0 https://github.com/baskaufs/guid-o-matic" ;
	<http://purl.org/dc/terms/modified> "2017-04-07T00:20:00.000Z"^^xsd:dateTime ;
	dc:creator "Biodiversity Information Standards (TDWG)" ;
	dc:format "text/turtle" .

<http://rs.tdwg.org/cv/status/uncertain> <http://purl.org/dc/terms/isPartOf> <http://rs.tdwg.org/cv/status/> ;
	a <http://www.w3.org/2004/02/skos/core#Concept> ;
	rdf:value "uncertain" ;
	rdfs:comment "A record exists of the species' presence in the area, but this record requires verification or is rendered questionable owing to uncertainty over the identity or authenticity of the record, or the accuracy of the location."@en ;
	rdfs:isDefinedBy <http://rs.tdwg.org/cv/status/> ;
	rdfs:label "presence uncertain"@en ;
	<http://www.w3.org/2004/02/skos/core#definition> "A record exists of the species' presence in the area, but this record requires verification or is rendered questionable owing to uncertainty over the identity or authenticity of the record, or the accuracy of the location."@en , "La presencia de la especie se ha registrado en el area, pero dicho registro necesita ser verificado o es cuestionable debido a la incertidumbre o autenticidad del registro o la exactitud de la localidad"@es , "Existe um registo de presença da espécie na área mas este registo necessita verificação, é duvidoso devido à sua incerta identidade ou autenticidade, ou devido à precisão da localidade."@pt , "有该物种在该区域存在的记录，但是该记录需要验证或者由于不确定其可识别性或真实性，抑或是不确定其位置的准确度而存疑。"@zh-hans , "有該物種在該區域存在的記錄，但是該記錄需要驗證或者由于不確定其可識別性或真實性，抑或是不確定其位置的准確度而存疑。"@zh-hant , "Eine Aufzeichnung von der Anwesenheit der Art in dem Gebiet existiert, aber die Aufzeichnung erfordert Verifizierung oder ist fragwürdig aufgrund von Unsicherheit bezüglich der Identität oder Authentizität der Aufzeichnung, oder Unsicherheit bezüglich der Genauigkeit der Lage. "@de ;
	<http://www.w3.org/2004/02/skos/core#hiddenLabel> "?" , "doubtful" , "doubtful (occurrence with \"0\" mark)." , "doubtful (occurrence with \"no\" mark)." , "doubtful (occurrence with \"x\" mark)." , "doubtful (occurrence with question mark)." , "Q" , "unclear breeding certaint" ;
	<http://www.w3.org/2004/02/skos/core#inScheme> <http://rs.tdwg.org/cv/status/> ;
	<http://www.w3.org/2004/02/skos/core#prefLabel> "presence uncertain"@en , "anwesenheit unsicher"@de , "presencia incierta"@es , "presença incerta"@pt , "存在未知"@zh-hans , "存在未知"@zh-hant .

<http://rs.tdwg.org/cv/status/uncertain.ttl> <http://purl.org/dc/terms/references> <http://rs.tdwg.org/cv/status/uncertain> ;
	a foaf:Document ;
	rdfs:comment "Generated by Guid-O-Matic 2.0 https://github.com/baskaufs/guid-o-matic" ;
	<http://purl.org/dc/terms/modified> "2017-04-07T00:20:00.000Z"^^xsd:dateTime ;
	dc:creator "Biodiversity Information Standards (TDWG)" ;
	dc:format "text/turtle" .

<http://rs.tdwg.org/cv/> <http://purl.org/dc/terms/license> <http://creativecommons.org/licenses/by/4.0/> ;
	<http://purl.org/dc/terms/isPartOf> <http://www.tdwg.org/standards/x> ;
	<http://purl.org/dc/terms/contributor> <http://orcid.org/0000-0003-4365-3135> , <http://orcid.org/0000-0002-0596-5376> ;
	<http://purl.org/dc/terms/bibliographicCitation> "placeholder for a future citation" ;
	<http://purl.org/dc/terms/hasPart> <http://rs.tdwg.org/cv/doe/> ;
	a <http://rs.tdwg.org/dwc/terms/attributes/Vocabulary> ;
	rdfs:comment "Draft; not part of any TDWG standard"@en ;
	rdfs:label "Establishment Means Controlled Vocabulary"@en ;
	<http://purl.org/dc/terms/description> "This vocabulary is under development to provide controlled vocabulary values for possible future Darwin Core terms that may extend or replace establishmentMeans."@en ;
	<http://purl.org/dc/terms/title> "Establishment Means Controlled Vocabulary"@en ;
	dc:creator "some task group not yet in existence" ;
	dc:contributor "Quentin Groom (Botanic Garden Meise)" , "Steve Baskauf (Vanderbilt University)" .

<http://rs.tdwg.org/cv/doe/> <http://purl.org/dc/terms/isPartOf> <http://rs.tdwg.org/cv/> ;
	<http://purl.org/vocab/vann/preferredNamespacePrefix> "cvdoe" ;
	<http://purl.org/vocab/vann/preferredNamespaceUri> "http://rs.tdwg.org/cv/doe/" ;
	a <http://rs.tdwg.org/dwc/terms/attributes/TermList> , <http://www.w3.org/2004/02/skos/core#ConceptScheme> ;
	rdfs:comment "For each term in this list, the controlled value (rdf:value), and definition (rdfs:comment) are normative.  Labels (rdfs:label) and comments (dcterms:description) are non-normative." , "This is a controlled vocabulary whose terms are intended to be used as values for a proposed Darwin Core term dwc:degreeOfEstablishment/dwciri:degreeOfEstablishment."@en ;
	rdfs:label "Degree of Establishment Controlled Vocabulary Term List"@en ;
	<http://www.w3.org/2004/02/skos/core#hasTopConcept> <http://rs.tdwg.org/cv/doe/A> , <http://rs.tdwg.org/cv/doe/B> , <http://rs.tdwg.org/cv/doe/C> , <http://rs.tdwg.org/cv/doe/D> , <http://rs.tdwg.org/cv/doe/E> ;
	<http://www.w3.org/2004/02/skos/core#note> "This is a controlled vocabulary whose terms are intended to be used as values for a proposed Darwin Core term dwc:degreeOfEstablishment/dwciri:degreeOfEstablishment."@en ;
	<http://purl.org/dc/terms/modified> "2017-04-06"^^xsd:date ;
	<http://purl.org/dc/terms/title> "Degree of Establishment Controlled Vocabulary Term List"@en .

<http://rs.tdwg.org/cv/origin/> <http://purl.org/dc/terms/isPartOf> <http://rs.tdwg.org/cv/> ;
	<http://purl.org/vocab/vann/preferredNamespacePrefix> "cvorigin" ;
	<http://purl.org/vocab/vann/preferredNamespaceUri> "http://rs.tdwg.org/cv/origin/" .

<http://rs.tdwg.org/cv/status/> <http://purl.org/dc/terms/isPartOf> <http://rs.tdwg.org/cv/> ;
	<http://purl.org/vocab/vann/preferredNamespacePrefix> "cvstatus" ;
	<http://purl.org/vocab/vann/preferredNamespaceUri> "http://rs.tdwg.org/cv/status/" ;
	a <http://rs.tdwg.org/dwc/terms/attributes/TermList> , <http://www.w3.org/2004/02/skos/core#ConceptScheme> ;
	rdfs:comment "For each term in this list, the controlled value (rdf:value), and definition (rdfs:comment) are normative.  Labels (rdfs:label) and comments (dcterms:description) are non-normative." , "This is a controlled vocabulary whose terms are intended to be used as values for a proposed Darwin Core term dwc:occurrenceStatus/dwciri:occurrenceStatus."@en ;
	rdfs:label "Occurrence Status Controlled Vocabulary Term List"@en ;
	<http://www.w3.org/2004/02/skos/core#hasTopConcept> <http://rs.tdwg.org/cv/status/absent> , <http://rs.tdwg.org/cv/status/extant> , <http://rs.tdwg.org/cv/status/extinct> , <http://rs.tdwg.org/cv/status/pextant> , <http://rs.tdwg.org/cv/status/pextinct> , <http://rs.tdwg.org/cv/status/uncertain> ;
	<http://www.w3.org/2004/02/skos/core#note> "This is a controlled vocabulary whose terms are intended to be used as values for a proposed Darwin Core term dwc:occurrenceStatus/dwciri:occurrenceStatus."@en ;
	<http://purl.org/dc/terms/modified> "2017-04-06"^^xsd:date ;
	<http://purl.org/dc/terms/title> "Occurrence Status Controlled Vocabulary Term List"@en .

<http://rs.tdwg.org/cv/status/absent> <http://purl.org/dc/terms/isPartOf> <http://rs.tdwg.org/cv/status/> ;
	a <http://www.w3.org/2004/02/skos/core#Concept> ;
	rdf:value "absent" ;
	rdfs:comment "Not present in a place at an occasion"@en ;
	rdfs:isDefinedBy <http://rs.tdwg.org/cv/status/> ;
	rdfs:label "absent"@en ;
	<http://www.w3.org/2004/02/skos/core#definition> "Not present in a place at an occasion"@en , "Nicht und noch nie in einem Gebiet anwesend. "@de , "No está presente en la localidad"@es , "Não presente num lugar num momento."@pt , "该物种在某些场合在某地区不存在"@zh-hans , "該物種在某些場合在某地區不存在。"@zh-hant ;
	<http://www.w3.org/2004/02/skos/core#hiddenLabel> "absent" , "Absent" , "Ausente" ;
	<http://www.w3.org/2004/02/skos/core#inScheme> <http://rs.tdwg.org/cv/status/> ;
	<http://www.w3.org/2004/02/skos/core#prefLabel> "absent"@en , "absent abwesend"@de , "ausente"@es , "ausente"@pt , "缺席"@zh-hans , "缺席"@zh-hant .

<http://rs.tdwg.org/cv/status/absent.ttl> <http://purl.org/dc/terms/references> <http://rs.tdwg.org/cv/status/absent> ;
	a foaf:Document ;
	rdfs:comment "Generated by Guid-O-Matic 2.0 https://github.com/baskaufs/guid-o-matic" ;
	<http://purl.org/dc/terms/modified> "2017-04-07T00:20:00.000Z"^^xsd:dateTime ;
	dc:creator "Biodiversity Information Standards (TDWG)" ;
	dc:format "text/turtle" .

<http://rs.tdwg.org/cv/status/extant> <http://purl.org/dc/terms/isPartOf> <http://rs.tdwg.org/cv/status/> ;
	a <http://www.w3.org/2004/02/skos/core#Concept> ;
	rdf:value "extant" ;
	rdfs:comment "The species is known or thought very likely to occur presently in the area, which encompasses localities with current or recent (last 20-30 years) records where suitable habitat at appropriate altitudes remains."@en ;
	rdfs:isDefinedBy <http://rs.tdwg.org/cv/status/> ;
	rdfs:label "extant"@en ;
	<http://www.w3.org/2004/02/skos/core#definition> "The species is known or thought very likely to occur presently in the area, which encompasses localities with current or recent (last 20-30 years) records where suitable habitat at appropriate altitudes remains."@en , "Von der Art ist bekannt oder wird mit hoher Wahrscheinlichkeit angenommen, dass sie derzeit im Gebiet anwesend ist, und für die Art existieren aktuelle oder in den letzten 20 bis 30 Jahren erstellte Aufzeichnungen, in Lagen mit geeigneten Lebensräumen. "@de , "Se conoce o espera con alta probabilidad que la especie se encuentre en el area, incluyendo localidades con registros recientes (los ultimos  20-30 años) de la presencia de un habitat adecuado a una altitud apropiada"@es , "Sabe-se que a espécie ocorre na área ou a sua ocorrência é tida como bastante provável, o que inclui localidades com registos atuais ou recentes (últimos 20-30 anos) nas quais se mantêm habitats adequados às altitudes apropriadas."@pt , "该物种在该地区存在或者很可能存在。该地区包括了在现在以及近些年间（20－30年）的记录中海拔适宜的栖息地仍然存在的地方。"@zh-hans , "該物種在該地區存在或者很可能存在。該地區包括了在現在以及近些年間（20－30年）的記錄中海拔適宜的棲息地仍然存在的地方。"@zh-hant ;
	<http://www.w3.org/2004/02/skos/core#hiddenLabel> "breeding in region" , "common" , "Común" , "confirmed breeding" , "frecuente" , "Frecuente" , "Infested" , "Irregular" , "Outbreak" , "P" , "presence" , "present" , "Present" , "Présent " , "presente" , "Presente" , "Raro" , "Reported" ;
	<http://www.w3.org/2004/02/skos/core#inScheme> <http://rs.tdwg.org/cv/status/> ;
	<http://www.w3.org/2004/02/skos/core#prefLabel> "extant"@en , "vorhanden "@de , "existente"@es , "presente"@pt , "现存"@zh-hans , "現存"@zh-hant .

<http://rs.tdwg.org/cv/status/extant.ttl> <http://purl.org/dc/terms/references> <http://rs.tdwg.org/cv/status/extant> ;
	a foaf:Document ;
	rdfs:comment "Generated by Guid-O-Matic 2.0 https://github.com/baskaufs/guid-o-matic" ;
	<http://purl.org/dc/terms/modified> "2017-04-07T00:20:00.000Z"^^xsd:dateTime ;
	dc:creator "Biodiversity Information Standards (TDWG)" ;
	dc:format "text/turtle" .

<http://rs.tdwg.org/cv/status/extinct> <http://purl.org/dc/terms/isPartOf> <http://rs.tdwg.org/cv/status/> ;
	a <http://www.w3.org/2004/02/skos/core#Concept> ;
	rdf:value "extinct" ;
	rdfs:comment "The species was formerly known or thought very likely to occur in the area, but it has been confirmed that the species no longer occurs because exhaustive searches have failed to produce recent records, and the intensity and timing of threats could plausibly have extirpated the taxon."@en ;
	rdfs:isDefinedBy <http://rs.tdwg.org/cv/status/> ;
	rdfs:label "extinct"@en ;
	<http://www.w3.org/2004/02/skos/core#definition> "该物种曾经在该区域存在过或者很可能存在过， 但是由于对该地区彻底调查后没有发现任何近期该物种出现的记录，并且其受到的威胁的强度和时机有根除该物种的可能性，该物种已经被确认不再存在。"@zh-hans , "該物種曾經在該區域存在過或者很可能存在過， 但是由于對該地區徹底調查後沒有發現任何近期該物種出現的記錄，並且其受到的威脅的強度和時機有根除該物種的可能性，該物種已經被確認不再存在。"@zh-hant , "Sabe-se que a espécie ocorreu na área ou a sua ocorrência foi tida como bastante provável mas confirmou-se que a espécie já não aí ocorre devido a procuras exaustivas serem incapazes de produzir registos recentes; a intensidade e timing das ameaças terá provavelmente extirpado o táxone."@pt , "Von der Art war früher bekannt oder wurde mit hoher Wahrscheinlichkeit angenommen, dass sie im Gebiet anwesend war, aber inzwischen wurde bestätigt, dass die Art dort nicht länger auftritt, aufgrund von gründlicher, aber vergeblicher, aktueller Suche, wobei es plausibel ist, dass das Taxon aufgrund der Intensität und des Zeitpunkts der Bedrohung ausgerottet sein dürfte."@de , "The species was formerly known or thought very likely to occur in the area, but it has been confirmed that the species no longer occurs because exhaustive searches have failed to produce recent records, and the intensity and timing of threats could plausibly have extirpated the taxon."@en , "Se sabe de la existencia de la especie en el area en el pasado, o se cree que la especie pudo haber existido en el area, pero se ha confirmado que la especie no se encuentra debido a que luego de búsquedas exhaustivas, no se han producido registros recientes, y la intensidad duracion de amenazas posiblemente hayan extirpado el taxón"@es .
